ranges in env context

pulse/lib/steel/pulse/Pulse.Checker.Abs.fst
@@ -21,6 +21,7 @@ let check_abs
   (check:check_t)
   : T.Tac (checker_result_t g pre post_hint) =
   if Some? post_hint then T.fail "Unexpected post-condition annotation from context for an abstraction" else 
+  let range = t.range in
   match t.term with  
   | Tm_Abs { b = {binder_ty=t;binder_ppname=ppname}; q=qual; pre=pre_hint; body; ret_ty; post=post_hint_body } ->
     (*  (fun (x:t) -> {pre_hint} body : t { post_hint } *)
@@ -43,7 +44,10 @@ let check_abs
         match post_hint_body with
         | None -> None
         | Some post ->
-          let post_hint_typing : post_hint_t = Pulse.Checker.Common.intro_post_hint (push_context "post_hint_typing" g') ret_ty post in
+          let post_hint_typing
+            : post_hint_t
+            = Pulse.Checker.Common.intro_post_hint (push_context "post_hint_typing" range g') ret_ty post
+          in
           Some post_hint_typing
       in
       let (| body', c_body, body_typing |) = check g' (open_st_term_nv body px) pre_opened (E pre_typing) post in
