pulse/lib/steel/pulse/Pulse.RuntimeUtils.fsti
@@ -1,8 +1,8 @@
 module Pulse.RuntimeUtils
 open FStar.Tactics
 module T = FStar.Tactics
-type context = FStar.Sealed.Inhabited.sealed #(list string) []
-val extend_context (tag:string) (ctx:context) : context
+type context = FStar.Sealed.Inhabited.sealed #(list (string & option range)) []
+val extend_context (tag:string) (r:option range) (ctx:context) : context
 val debug_at_level (g:env) (s:string) : bool
 val print_exn (e:exn) : string
 val bv_set_range (x:bv) (r:range) : b:bv{b==x}
