pulse/lib/steel/pulse/Pulse.Checker.Rewrite.fst
@@ -17,7 +17,7 @@ let check_rewrite
   (pre_typing:tot_typing g pre Tm_VProp)
   (post_hint:post_hint_opt g)
   : T.Tac (checker_result_t g pre post_hint) =
-  let g = push_context "check_rewrite" g in
+  let g = push_context "check_rewrite" t.range g in
   let Tm_Rewrite {t1=p; t2=q} = t.term in
   let (| p, p_typing |) = check_vprop g p in
   let (| q, q_typing |) = check_vprop g q in
