pulse/lib/steel/pulse/Pulse.Checker.WithLocal.fst
@@ -35,7 +35,7 @@ let check_withlocal
   (post_hint:post_hint_opt g)
   (check':bool -> check_t)
   : T.Tac (checker_result_t g pre post_hint) =
-  let g = push_context "check_withlocal" g in
+  let g = push_context "check_withlocal" t.range g in
   let wr t0 = { term = t0; range = t.range } in
   let Tm_WithLocal {binder; initializer=init; body} = t.term in
   let (| init, init_u, init_t, init_t_typing, init_typing |) =
