pulse/lib/steel/pulse/Pulse.Typing.Env.fsti
@@ -7,7 +7,7 @@ open Pulse.Syntax
 module L = FStar.List.Tot
 
 module RT = FStar.Reflection.Typing
-
+module T = FStar.Tactics
 val env : Type0
 
 val fstar_env (g:env) : RT.fstar_top_env
@@ -126,6 +126,7 @@ val extends_with_push (g1 g2 g3:env)
            SMTPat (push_binding g1 x t);
            SMTPat (push_binding g3 x t)]
 
-val push_context (g:env) (ctx:string) : g':env { g' == g }
-
+val push_context (g:env) (ctx:string) (r:range) : g':env { g' == g }
+val push_context_no_range (g:env) (ctx:string) : g':env { g' == g }
 val get_context (g:env) : Pulse.RuntimeUtils.context
+val range_of_env (g:env) : T.Tac range
